src/program_proof/wal/circ_proof.v
@@ -164,6 +164,16 @@ Proof.
   word.
 Qed.
 
+Theorem start_is_to_at_least (γ: circ_names) (x: u64) q :
+  start_is γ q x -∗
+  |==> start_is γ q x ∗ start_at_least γ x.
+Proof.
+  iIntros "H".
+  iMod (fmcounter_get_lb with "H") as "[H Hlb]".
+  iFrame.
+  auto.
+Qed.
+
 Instance diskEnd_fractional γ endpos : Fractional (λ q, diskEnd_is γ q endpos).
 Proof.
   intros p q.
